src/ocaml/bitblasting/bitblasting.mli
@@ -9,11 +9,13 @@ type vm = ssavar M.t
 
 val option_debug : bool ref
 
+val option_split_conjs : bool ref
+
 val string_of_exp : QFBV.exp -> string
 
 val string_of_bexp : QFBV.bexp -> string
 
-val bexp_of_file : file -> vm * tm * SSATE.env * QFBV.bexp
+val bexps_of_file : file -> vm * tm * SSATE.env * QFBV.bexp list
 
 val bb_file : file -> cnf
 
