src/bbcache/CacheFlatten.v
@@ -1,6 +1,6 @@
 From Coq Require Import ZArith OrderedType Bool.
 From mathcomp Require Import ssreflect ssrfun ssrbool ssrnat eqtype seq tuple fintype choice.
-From ssrlib Require Import FMaps Var.
+From ssrlib Require Import FMaps Var Seqs Tactics.
 From BitBlasting Require Import QFBV CNF State BBCommon.
 From BBCache Require Import CompTableFlatten SimpTable CompCache.
 
@@ -48,3 +48,222 @@ Definition add_cbt e l c :=
 Definition reset_ct (c : cache) :=
   {| ht := ht c;
      ct := SimpTable.empty |}.
+
+
+(* Cache compatible *)
+
+From BBCache Require Cache.
+
+Definition ct_equal fc c := SimpTable.Equal (ct fc) (Cache.ct c).
+
+Definition ht_compatible fc c := comptable_compatible (ht fc) (Cache.ht c).
+
+Definition cache_compatible ec c := ct_equal ec c /\ ht_compatible ec c.
+
+Lemma cache_compatible_reset_ct ec c :
+  cache_compatible ec c -> cache_compatible (reset_ct ec)
+                                            (Cache.reset_ct c).
+Proof.
+  move=> [[Hct_e Hct_b] [Hht_e Hht_b]]. split; [split | split].
+  - rewrite /reset_ct /=. reflexivity.
+  - rewrite /reset_ct /=. reflexivity.
+  - assumption.
+  - assumption.
+Qed.
+
+Lemma cache_compatible_find_cet ec c e :
+  cache_compatible ec c -> find_cet e ec = Cache.find_cet e c.
+Proof.
+  move=> [[Hct_e Hct_b] _]. rewrite /find_cet /SimpTable.find_et.
+  rewrite (Hct_e e). reflexivity.
+Qed.
+
+Lemma cache_compatible_find_cbt ec c e :
+  cache_compatible ec c -> find_cbt e ec = Cache.find_cbt e c.
+Proof.
+  move=> [[Hct_e Hct_b] _]. rewrite /find_cbt /SimpTable.find_bt.
+  rewrite (Hct_b e). reflexivity.
+Qed.
+
+Lemma cache_compatible_find_het_none ec c e :
+  cache_compatible ec c ->
+  (find_het e ec = None <-> Cache.find_het e c = None).
+Proof.
+  move=> [_ [Hht_e Hht_b]]. rewrite /find_het /CompTableFlatten.find_et.
+  rewrite /Cache.find_het /CompTable.find_et. move: (Hht_e e) => [H1 H2].
+  split=> H.
+  - apply: CompTable.ExpMap.Lemmas.not_mem_find_none. rewrite -H1. apply/negPf.
+    apply: CompTableFlatten.ExpMap.Lemmas.find_none_not_mem. assumption.
+  - apply: CompTableFlatten.ExpMap.Lemmas.not_mem_find_none.
+    rewrite H1. apply/negPf. apply: CompTable.ExpMap.Lemmas.find_none_not_mem.
+    assumption.
+Qed.
+
+Lemma cache_compatible_find_hbt_none ec c e :
+  cache_compatible ec c ->
+  (find_hbt e ec = None <-> Cache.find_hbt e c = None).
+Proof.
+  move=> [_ [Hht_e Hht_b]]. rewrite /find_hbt /CompTableFlatten.find_bt.
+  rewrite /Cache.find_hbt /CompTable.find_bt. move: (Hht_b e) => [H1 H2].
+  split=> H.
+  - apply: CompTable.BexpMap.Lemmas.not_mem_find_none. rewrite -H1. apply/negPf.
+    apply: CompTableFlatten.BexpMap.Lemmas.find_none_not_mem. assumption.
+  - apply: CompTableFlatten.BexpMap.Lemmas.not_mem_find_none.
+    rewrite H1. apply/negPf. apply: CompTable.BexpMap.Lemmas.find_none_not_mem.
+    assumption.
+Qed.
+
+Lemma cache_compatible_find_het_some ec c e ecs elrs cs lrs :
+  cache_compatible ec c ->
+  find_het e ec = Some (ecs, elrs) ->
+  Cache.find_het e c = Some (cs, lrs) ->
+  cnf_eqsat (tflatten ecs) cs /\ elrs = lrs.
+Proof.
+  move=> [_ [Hht_e Hht_b]] Hfe Hf. move: (Hht_e e) => [H1 H2].
+  exact: (H2 _ _ _ _ Hfe Hf).
+Qed.
+
+Lemma cache_compatible_find_het_some_exists1 ec c e ecs elrs :
+  cache_compatible ec c ->
+  find_het e ec = Some (ecs, elrs) ->
+  exists cs, Cache.find_het e c = Some (cs, elrs) /\
+             cnf_eqsat (tflatten ecs) cs.
+Proof.
+  move=> Hcc Hfe. dcase (Cache.find_het e c); case.
+  - move=> [cs lrs] Hf. move: (cache_compatible_find_het_some Hcc Hfe Hf) => [H1 H2].
+    exists cs. rewrite H2. done.
+  - move=> Hf. move/(cache_compatible_find_het_none _ Hcc): Hf. rewrite Hfe.
+    discriminate.
+Qed.
+
+Lemma cache_compatible_find_het_some_exists2 ec c e cs lrs :
+  cache_compatible ec c ->
+  Cache.find_het e c = Some (cs, lrs) ->
+  exists ecs, find_het e ec = Some (ecs, lrs) /\
+             cnf_eqsat (tflatten ecs) cs.
+Proof.
+  move=> Hcc Hf. dcase (find_het e ec); case.
+  - move=> [ecs elrs] Hfe.
+    move: (cache_compatible_find_het_some Hcc Hfe Hf) => [H1 H2].
+    exists ecs. rewrite H2. done.
+  - move=> Hfe. move/(cache_compatible_find_het_none _ Hcc): Hfe. rewrite Hf.
+    discriminate.
+Qed.
+
+Lemma cache_compatible_find_hbt_some ec c e ecs elr cs lr :
+  cache_compatible ec c ->
+  find_hbt e ec = Some (ecs, elr) ->
+  Cache.find_hbt e c = Some (cs, lr) ->
+  cnf_eqsat (tflatten ecs) cs /\ elr = lr.
+Proof.
+  move=> [_ [Hht_e Hht_b]] Hfe Hf. move: (Hht_b e) => [H1 H2].
+  exact: (H2 _ _ _ _ Hfe Hf).
+Qed.
+
+Lemma cache_compatible_find_hbt_some_exists1 ec c e ecs elr :
+  cache_compatible ec c ->
+  find_hbt e ec = Some (ecs, elr) ->
+  exists cs, Cache.find_hbt e c = Some (cs, elr) /\
+             cnf_eqsat (tflatten ecs) cs.
+Proof.
+  move=> Hcc Hfe. dcase (Cache.find_hbt e c); case.
+  - move=> [cs lrs] Hf. move: (cache_compatible_find_hbt_some Hcc Hfe Hf) => [H1 H2].
+    exists cs. rewrite H2. done.
+  - move=> Hf. move/(cache_compatible_find_hbt_none _ Hcc): Hf. rewrite Hfe.
+    discriminate.
+Qed.
+
+Lemma cache_compatible_find_hbt_some_exists2 ec c e cs lr :
+  cache_compatible ec c ->
+  Cache.find_hbt e c = Some (cs, lr) ->
+  exists ecs, find_hbt e ec = Some (ecs, lr) /\
+             cnf_eqsat (tflatten ecs) cs.
+Proof.
+  move=> Hcc Hf. dcase (find_hbt e ec); case.
+  - move=> [ecs elrs] Hfe.
+    move: (cache_compatible_find_hbt_some Hcc Hfe Hf) => [H1 H2].
+    exists ecs. rewrite H2. done.
+  - move=> Hfe. move/(cache_compatible_find_hbt_none _ Hcc): Hfe. rewrite Hf.
+    discriminate.
+Qed.
+
+Lemma cache_compatible_add_cet e lrs ec c :
+  cache_compatible ec c ->
+  cache_compatible (add_cet e lrs ec) (Cache.add_cet e lrs c).
+Proof.
+  move=> [[Hcet Hcbt] [Hhet Hhbt]]. split; [split | split].
+  - rewrite /add_cet /Cache.add_cet /=. by apply: CompTable.ExpMap.Lemmas.add_m.
+  - assumption.
+  - assumption.
+  - assumption.
+Qed.
+
+Lemma cache_compatible_add_cbt e lr ec c :
+  cache_compatible ec c ->
+  cache_compatible (add_cbt e lr ec) (Cache.add_cbt e lr c).
+Proof.
+  move=> [[Hcet Hcbt] [Hhet Hhbt]]. split; [split | split].
+  - assumption.
+  - rewrite /add_cbt /Cache.add_cbt /=. by apply: CompTable.BexpMap.Lemmas.add_m.
+  - assumption.
+  - assumption.
+Qed.
+
+Lemma cache_compatible_add_het e lrs ec c ecs cs :
+  cache_compatible ec c ->
+  cnf_eqsat (tflatten ecs) cs ->
+  cache_compatible (add_het e ecs lrs ec) (Cache.add_het e cs lrs c).
+Proof.
+  move=> [[Hcet Hcbt] [Hhet Hhbt]] Heqs. split; [split | split].
+  - assumption.
+  - assumption.
+  - rewrite /add_het /Cache.add_het /=. move=> f. move: (Hhet f) => [H1 H2].
+    split.
+    + rewrite CompTableFlatten.ExpMap.Lemmas.add_b.
+      rewrite CompTable.ExpMap.Lemmas.add_b.
+      rewrite H1. reflexivity.
+    + move=> ecs' elrs' cs' lrs'.
+      rewrite CompTableFlatten.ExpMap.Lemmas.add_o.
+      rewrite CompTable.ExpMap.Lemmas.add_o.
+      case: (CompTableFlatten.ExpMap.M.E.eq_dec e f);
+        case: (CompTable.ExpMap.M.E.eq_dec e f) => //=.
+      * move=> /eqP Hef _ [] ? ? [] ? ?; subst. done.
+      * move=> _ _ Hfe Hf. exact: (H2 _ _ _ _ Hfe Hf).
+  - assumption.
+Qed.
+
+Lemma cache_compatible_add_hbt e lr ec c ecs cs :
+  cache_compatible ec c ->
+  cnf_eqsat (tflatten ecs) cs ->
+  cache_compatible (add_hbt e ecs lr ec) (Cache.add_hbt e cs lr c).
+Proof.
+  move=> [[Hcet Hcbt] [Hhet Hhbt]] Heqs. split; [split | split].
+  - assumption.
+  - assumption.
+  - assumption.
+  - rewrite /add_hbt /Cache.add_hbt /=. move=> f. move: (Hhbt f) => [H1 H2].
+    split.
+    + rewrite CompTableFlatten.BexpMap.Lemmas.add_b.
+      rewrite CompTable.BexpMap.Lemmas.add_b.
+      rewrite H1. reflexivity.
+    + move=> ecs' elr' cs' lr'.
+      rewrite CompTableFlatten.BexpMap.Lemmas.add_o.
+      rewrite CompTable.BexpMap.Lemmas.add_o.
+      case: (CompTableFlatten.BexpMap.M.E.eq_dec e f);
+        case: (CompTable.BexpMap.M.E.eq_dec e f) => //=.
+      * move=> /eqP Hef _ [] ? ? [] ? ?; subst. done.
+      * move=> _ _ Hfe Hf. exact: (H2 _ _ _ _ Hfe Hf).
+Qed.
+
+
+(* Convert CacheFlatten to Cache *)
+
+Definition cache_of_fcache (c : cache) : Cache.cache :=
+  Cache.Build_cache (comptable_of_fcomptable (ht c))
+                    (ct c).
+
+Lemma cache_of_fcache_compatible fc :
+  cache_compatible fc (cache_of_fcache fc).
+Proof.
+  split; [split; reflexivity | exact: comptable_of_fcomptable_compatible].
+Qed.
