src/bbcache/CacheHash.v
@@ -48,3 +48,280 @@ Definition add_cbt e l c :=
 Definition reset_ct (c : cache) :=
   {| ht := ht c;
      ct := SimpTableHash.empty |}.
+
+
+
+
+From BBCache Require SimpTable CompTableFlatten CacheFlatten.
+
+Section CacheCompatible.
+
+  Import QFBV.
+
+  Definition cet_compatible
+             (ht : SimpTableHash.simptable) (ft : SimpTable.simptable) : Prop :=
+    forall (e : exp),
+      SimpTableHash.find_et (hash_exp e) ht = SimpTable.find_et e ft.
+
+  Definition cbt_compatible
+             (ht : SimpTableHash.simptable) (ft : SimpTable.simptable) : Prop :=
+    forall (e : bexp),
+      SimpTableHash.find_bt (hash_bexp e) ht = SimpTable.find_bt e ft.
+
+  Definition ct_compatible
+             (ht : SimpTableHash.simptable) (ft : SimpTable.simptable) : Prop :=
+    cet_compatible ht ft /\ cbt_compatible ht ft.
+
+  Definition het_compatible
+             (ht : CompTableHash.comptable) (ft : CompTableFlatten.comptable) : Prop :=
+    forall (e : exp),
+      CompTableHash.find_et (hash_exp e) ht = CompTableFlatten.find_et e ft.
+
+  Definition hbt_compatible
+             (ht : CompTableHash.comptable) (ft : CompTableFlatten.comptable) : Prop :=
+    forall (e : bexp),
+      CompTableHash.find_bt (hash_bexp e) ht = CompTableFlatten.find_bt e ft.
+
+  Definition ht_compatible
+             (ht : CompTableHash.comptable) (ft : CompTableFlatten.comptable) : Prop :=
+    het_compatible ht ft /\ hbt_compatible ht ft.
+
+  Definition cache_compatible
+             (hc : cache) (fc : CacheFlatten.cache) : Prop :=
+    ct_compatible (ct hc) (CacheFlatten.ct fc) /\
+    ht_compatible (ht hc) (CacheFlatten.ht fc).
+
+  Lemma cache_compatible_find_cet hc fc (e : exp) :
+    cache_compatible hc fc ->
+    find_cet (hash_exp e) hc = CacheFlatten.find_cet e fc.
+  Proof. move=>[[H1 H2] [H3 H4]]. exact: (H1 e). Qed.
+
+  Lemma cache_compatible_find_cbt hc fc (e : bexp) :
+    cache_compatible hc fc ->
+    find_cbt (hash_bexp e) hc = CacheFlatten.find_cbt e fc.
+  Proof. move=>[[H1 H2] [H3 H4]]. exact: (H2 e). Qed.
+
+  Lemma cache_compatible_find_het hc fc (e : exp) :
+    cache_compatible hc fc ->
+    find_het (hash_exp e) hc = CacheFlatten.find_het e fc.
+  Proof. move=>[[H1 H2] [H3 H4]]. exact: (H3 e). Qed.
+
+  Lemma cache_compatible_find_hbt hc fc (e : bexp) :
+    cache_compatible hc fc ->
+    find_hbt (hash_bexp e) hc = CacheFlatten.find_hbt e fc.
+  Proof. move=>[[H1 H2] [H3 H4]]. exact: (H4 e). Qed.
+
+  Lemma cache_compatible_find_cet_hexp hc fc (e : hexp) :
+    cache_compatible hc fc ->
+    well_formed_hexp e ->
+    find_cet e hc = CacheFlatten.find_cet e fc.
+  Proof.
+    move=> Hcc Hwf. rewrite -{1}(hash_unhash_hexp Hwf).
+    exact: (cache_compatible_find_cet _ Hcc).
+  Qed.
+
+  Lemma cache_compatible_find_cbt_hbexp hc fc (e : hbexp) :
+    cache_compatible hc fc ->
+    well_formed_hbexp e ->
+    find_cbt e hc = CacheFlatten.find_cbt e fc.
+  Proof.
+    move=> Hcc Hwf. rewrite -{1}(hash_unhash_hbexp Hwf).
+    exact: (cache_compatible_find_cbt _ Hcc).
+  Qed.
+
+  Lemma cache_compatible_find_het_hexp hc fc (e : hexp) :
+    cache_compatible hc fc ->
+    well_formed_hexp e ->
+    find_het e hc = CacheFlatten.find_het e fc.
+  Proof.
+    move=> Hcc Hwf. rewrite -{1}(hash_unhash_hexp Hwf).
+    exact: (cache_compatible_find_het _ Hcc).
+  Qed.
+
+  Lemma cache_compatible_find_hbt_hbexp hc fc (e : hbexp) :
+    cache_compatible hc fc ->
+    well_formed_hbexp e ->
+    find_hbt e hc = CacheFlatten.find_hbt e fc.
+  Proof.
+    move=> Hcc Hwf. rewrite -{1}(hash_unhash_hbexp Hwf).
+    exact: (cache_compatible_find_hbt _ Hcc).
+  Qed.
+
+  Lemma cache_compatible_add_cet hc fc (e : exp) ls :
+    cache_compatible hc fc ->
+    cache_compatible (add_cet (hash_exp e) ls hc)
+                     (CacheFlatten.add_cet e ls fc).
+  Proof.
+    move=> [[H1 H2] [H3 H4]]. repeat split => //=.
+    move=> f. case Heq: (f == e).
+    - rewrite (eqP Heq) SimpTableHash.find_et_add_et_eq SimpTable.find_et_add_et_eq.
+      reflexivity.
+    - move/negP: Heq => Hne.
+      have Hne_hexp: ~ hash_exp f == hash_exp e.
+      { move=> /eqP H; apply: Hne. apply/eqP. exact: (hash_exp_inj H). }
+      rewrite (SimpTableHash.find_et_add_et_neq _ _ Hne_hexp).
+      rewrite (SimpTable.find_et_add_et_neq _ _ Hne).
+      exact: (H1 f).
+  Qed.
+
+  Lemma cache_compatible_add_cbt hc fc (e : bexp) ls :
+    cache_compatible hc fc ->
+    cache_compatible (add_cbt (hash_bexp e) ls hc)
+                     (CacheFlatten.add_cbt e ls fc).
+  Proof.
+    move=> [[H1 H2] [H3 H4]]. repeat split => //=.
+    move=> f. case Heq: (f == e).
+    - rewrite (eqP Heq) SimpTableHash.find_bt_add_bt_eq SimpTable.find_bt_add_bt_eq.
+      reflexivity.
+    - move/negP: Heq => Hne.
+      have Hne_hbexp: ~ hash_bexp f == hash_bexp e.
+      { move=> /eqP H; apply: Hne. apply/eqP. exact: (hash_bexp_inj H). }
+      rewrite (SimpTableHash.find_bt_add_bt_neq _ _ Hne_hbexp).
+      rewrite (SimpTable.find_bt_add_bt_neq _ _ Hne).
+      exact: (H2 f).
+  Qed.
+
+  Lemma cache_compatible_add_het hc fc (e : exp) cs ls :
+    cache_compatible hc fc ->
+    cache_compatible (add_het (hash_exp e) cs ls hc)
+                     (CacheFlatten.add_het e cs ls fc).
+  Proof.
+    move=> [[H1 H2] [H3 H4]]. repeat split => //=.
+    move=> f. case Heq: (f == e).
+    - rewrite (eqP Heq) CompTableHash.find_et_add_et_eq
+              CompTableFlatten.find_et_add_et_eq.
+      reflexivity.
+    - move/negP: Heq => Hne.
+      have Hne_hexp: ~ hash_exp f == hash_exp e.
+      { move=> /eqP H; apply: Hne. apply/eqP. exact: (hash_exp_inj H). }
+      rewrite (CompTableHash.find_et_add_et_neq _ _ _ Hne_hexp).
+      rewrite (CompTableFlatten.find_et_add_et_neq _ _ _ Hne).
+      exact: (H3 f).
+  Qed.
+
+  Lemma cache_compatible_add_hbt hc fc (e : bexp) cs ls :
+    cache_compatible hc fc ->
+    cache_compatible (add_hbt (hash_bexp e) cs ls hc)
+                     (CacheFlatten.add_hbt e cs ls fc).
+  Proof.
+    move=> [[H1 H2] [H3 H4]]. repeat split => //=.
+    move=> f. case Heq: (f == e).
+    - rewrite (eqP Heq) CompTableHash.find_bt_add_bt_eq
+              CompTableFlatten.find_bt_add_bt_eq.
+      reflexivity.
+    - move/negP: Heq => Hne.
+      have Hne_hbexp: ~ hash_bexp f == hash_bexp e.
+      { move=> /eqP H; apply: Hne. apply/eqP. exact: (hash_bexp_inj H). }
+      rewrite (CompTableHash.find_bt_add_bt_neq _ _ _ Hne_hbexp).
+      rewrite (CompTableFlatten.find_bt_add_bt_neq _ _ _ Hne).
+      exact: (H4 f).
+  Qed.
+
+  Lemma cache_compatible_add_cet_hexp hc fc (e : hexp) ls :
+    cache_compatible hc fc ->
+    well_formed_hexp e ->
+    cache_compatible (add_cet e ls hc)
+                     (CacheFlatten.add_cet e ls fc).
+  Proof.
+    move=> Hcc Hwf. rewrite -{1}(hash_unhash_hexp Hwf).
+    exact: (cache_compatible_add_cet _ _ Hcc).
+  Qed.
+
+  Lemma cache_compatible_add_cet_hbexp hc fc (e : hbexp) ls :
+    cache_compatible hc fc ->
+    well_formed_hbexp e ->
+    cache_compatible (add_cbt e ls hc)
+                     (CacheFlatten.add_cbt e ls fc).
+  Proof.
+    move=> Hcc Hwf. rewrite -{1}(hash_unhash_hbexp Hwf).
+    exact: (cache_compatible_add_cbt _ _ Hcc).
+  Qed.
+
+  Lemma cache_compatible_reset_ct hc fc :
+    cache_compatible hc fc ->
+    cache_compatible (reset_ct hc) (CacheFlatten.reset_ct fc).
+  Proof.
+    rewrite /reset_ct /CacheFlatten.reset_ct. move=> [[H1 H2] [H3 H4]].
+      by repeat split.
+  Qed.
+
+End CacheCompatible.
+
+(*
+Section CacheConversion.
+
+  Definition comp_add_exp he v (m : CompTableFlatten.expm) :=
+    CompTableFlatten.ExpMap.add (QFBVHash.unhash_hexp he) v m.
+
+  Definition comp_add_bexp he v (m : CompTableFlatten.bexpm) :=
+    CompTableFlatten.BexpMap.add (QFBVHash.unhash_hbexp he) v m.
+
+  Definition hexpmap_of_expmap_comp (m : CompTableHash.expm) :
+    CompTableFlatten.expm :=
+    HexpMap.fold comp_add_exp m (CompTableFlatten.ExpMap.empty (seq cnf * word)).
+
+  Definition hbexpmap_of_bexpmap_comp (m : CompTableHash.bexpm) :
+    CompTableFlatten.bexpm :=
+    HbexpMap.fold comp_add_bexp m (CompTableFlatten.BexpMap.empty (seq cnf * literal)).
+
+  Definition fcomp_table_of_hcomp_table (m : CompTableHash.comptable) :
+    CompTableFlatten.comptable :=
+    CompTableFlatten.Build_comptable
+      (hexpmap_of_expmap_comp (CompTableHash.et m))
+      (hbexpmap_of_bexpmap_comp (CompTableHash.bt m)).
+
+  Definition simp_add_exp he v (m : SimpTable.expm) :=
+    CompTable.ExpMap.add (QFBVHash.unhash_hexp he) v m.
+
+  Definition simp_add_bexp he v (m : SimpTable.bexpm) :=
+    CompTable.BexpMap.add (QFBVHash.unhash_hbexp he) v m.
+
+  Definition hexpmap_of_expmap_simp (m : SimpTableHash.expm) :
+    SimpTable.expm :=
+    HexpMap.fold simp_add_exp m (CompTable.ExpMap.empty word).
+
+  Definition hbexpmap_of_bexpmap_simp (m : SimpTableHash.bexpm) :
+    SimpTable.bexpm :=
+    HbexpMap.fold simp_add_bexp m (CompTable.BexpMap.empty literal).
+
+  Definition fsimp_table_of_hsimp_table (m : SimpTableHash.simptable) :
+    SimpTable.simptable :=
+    SimpTable.Build_simptable
+      (hexpmap_of_expmap_simp (SimpTableHash.et m))
+      (hbexpmap_of_bexpmap_simp (SimpTableHash.bt m)).
+
+  Definition fcache_of_hcache (c : cache) : CacheFlatten.cache :=
+    CacheFlatten.Build_cache (fcomp_table_of_hcomp_table (ht c))
+                              (fsimp_table_of_hsimp_table (ct c)).
+
+  Lemma fsimp_table_of_hsimp_table_find_et c :
+    forall e : QFBV.exp,
+      find_et (hash_exp e) (ct c) =
+      SimpTable.find_et e (fsimp_table_of_hsimp_table (ct c)).
+  Proof.
+    move=> e. rewrite /fsimp_table_of_hsimp_table /SimpTable.find_et /=.
+    rewrite /find_et. rewrite /hexpmap_of_expmap_simp.
+    move: (et (ct c)) => {c} m. move: m.
+    eapply (@CompTableHash.HexpMap.Lemmas.OP.P.map_induction
+              word
+              (fun m =>
+                 HexpMap.find (hash_exp e) m =
+                 CompTable.ExpMap.find
+                   e
+                   (HexpMap.fold simp_add_exp m (CompTable.ExpMap.empty word)))).
+    - move=> m Hempty. 
+    -
+
+  Qed.
+  
+  Lemma fcache_of_hcache_compatible c : cache_compatible c (fcache_of_hcache c).
+  Proof.
+    split.
+    - split.
+      rewrite /fcache_of_hcache /cet_compatible /=.
+      
+    -
+  Qed.
+End CacheConversion
+*)
+
