src/Extract.v
@@ -24,7 +24,7 @@ Separate Extraction
          QFBV.well_formed_bexp QFBV.well_formed_bexps
          init_vm init_gen init_hcache CacheHash.reset_ct
          QFBVHash.hash_exp QFBVHash.hash_bexp QFBVHash.unhash_hashed_exp QFBVHash.unhash_hashed_bexp
-         bit_blast_bexp_hcache_tflatten
+         bit_blast_bexp_hcache bit_blast_bexp_hcache_tflatten bit_blast_bexps_hcache_conjs
          Seqs.tflatten add_prelude
          max_var_of_cnf num_clauses dimacs_cnf_with_header.
 Cd "../../..".
