src/bbcache/Cache.v
@@ -1,6 +1,6 @@
 From Coq Require Import ZArith OrderedType Bool.
 From mathcomp Require Import ssreflect ssrfun ssrbool ssrnat eqtype seq tuple fintype choice.
-From ssrlib Require Import FMaps Var. 
+From ssrlib Require Import FMaps Var.
 From BitBlasting Require Import QFBV CNF State BBCommon.
 From BBCache Require Import CompTable SimpTable CompCache.
 
@@ -22,26 +22,26 @@ Definition empty : cache :=
      ct := SimpTable.empty |}.
 
 Definition find_het e c := CompTable.find_et e (ht c).
-Definition find_hbt e c := CompTable.find_bt e (ht c). 
-Definition find_cet e c := SimpTable.find_et e (ct c). 
-Definition find_cbt e c := SimpTable.find_bt e (ct c). 
+Definition find_hbt e c := CompTable.find_bt e (ht c).
+Definition find_cet e c := SimpTable.find_et e (ct c).
+Definition find_cbt e c := SimpTable.find_bt e (ct c).
 
 
 (* ==== modification ==== *)
 
-Definition add_het e cs ls c := 
+Definition add_het e cs ls c :=
   {| ht := CompTable.add_et e cs ls (ht c);
      ct := ct c |}.
 
-Definition add_hbt e cs l c := 
+Definition add_hbt e cs l c :=
   {| ht := CompTable.add_bt e cs l (ht c);
      ct := ct c |}.
 
-Definition add_cet e ls c := 
+Definition add_cet e ls c :=
   {| ht := ht c;
      ct := SimpTable.add_et e ls (ct c) |}.
 
-Definition add_cbt e l c := 
+Definition add_cbt e l c :=
   {| ht := ht c;
      ct := SimpTable.add_bt e l (ct c) |}.
 
@@ -53,12 +53,12 @@ Definition reset_ct (c : cache) :=
 (* ==== compatible ==== *)
 
 Definition compatible (c1 : cache) (c2 : compcache) :=
-  SimpTable.compatible (ct c1) (CompCache.ct c2) 
+  SimpTable.compatible (ct c1) (CompCache.ct c2)
   /\ (ht c1) = (CompCache.ht c2).
 
 Lemma compatible_find_het :
   forall c1 c2 e, compatible c1 c2 -> find_het e c1 = CompCache.find_het e c2.
-Proof. 
+Proof.
   move=> c1 c2 e [Hct Hht] /=. rewrite /find_het Hht. done.
 Qed.
 
@@ -70,9 +70,9 @@ Qed.
 
 Lemma compatible_find_cet_some :
   forall c1 c2 e ls,
-    compatible c1 c2 -> find_cet e c1 = Some ls 
+    compatible c1 c2 -> find_cet e c1 = Some ls
     -> exists cs, CompCache.find_cet e c2 = Some (cs, ls).
-Proof. 
+Proof.
   move=> c1 c2 e ls [Hct Hht] /=. exact: SimpTable.compatible_find_et_some.
 Qed.
 
@@ -85,7 +85,7 @@ Qed.
 
 Lemma compatible_find_cbt_some :
   forall c1 c2 e l,
-    compatible c1 c2 -> find_cbt e c1 = Some l 
+    compatible c1 c2 -> find_cbt e c1 = Some l
     -> exists cs, CompCache.find_cbt e c2 = Some (cs, l).
 Proof.
   move=> c1 c2 e l [Hct Hht] /=. exact: SimpTable.compatible_find_bt_some.
@@ -100,7 +100,7 @@ Qed.
 
 Lemma compatible_add_het :
   forall c1 c2 e cs ls,
-    compatible c1 c2 
+    compatible c1 c2
     -> compatible (add_het e cs ls c1) (CompCache.add_het e cs ls c2).
 Proof.
   move=> c1 c2 e cs ls [Hct Hht]. split; [ done | by rewrite /add_het Hht ].
@@ -108,7 +108,7 @@ Qed.
 
 Lemma compatible_add_hbt :
   forall c1 c2 e cs l,
-    compatible c1 c2 
+    compatible c1 c2
     -> compatible (add_hbt e cs l c1) (CompCache.add_hbt e cs l c2).
 Proof.
   move=> c1 c2 e cs l [Hct Hht]. split; [ done | by rewrite /add_hbt Hht ].
@@ -118,7 +118,7 @@ Lemma compatible_add_cet :
   forall c1 c2 e cs ls,
     compatible c1 c2 -> compatible (add_cet e ls c1) (CompCache.add_cet e cs ls c2).
 Proof.
-  move=> c1 c2 e cs ls [Hct Hht]. 
+  move=> c1 c2 e cs ls [Hct Hht].
   split; [ exact: SimpTable.compatible_add_et | done ].
 Qed.
 
@@ -126,12 +126,12 @@ Lemma compatible_add_cbt :
   forall c1 c2 e cs l,
     compatible c1 c2 -> compatible (add_cbt e l c1) (CompCache.add_cbt e cs l c2).
 Proof.
-  move=> c1 c2 e cs ls [Hct Hht]. 
+  move=> c1 c2 e cs ls [Hct Hht].
   split; [ exact: SimpTable.compatible_add_bt | done ].
 Qed.
 
 Lemma compatible_reset_ct :
-  forall c1 c2, 
+  forall c1 c2,
     compatible c1 c2 -> compatible (reset_ct c1) (CompCache.reset_ct c2).
 Proof.
   move=> c1 c2 [Hct Hht]. split; done.
